Rename file system fields to make more sense:   files -> inode_tbl   file_inode -> files

basis/TextIOProofScript.sml
@@ -68,8 +68,8 @@ val STDIO_bumpFD = Q.store_thm("STDIO_bumpFD[simp]",
 val UNIQUE_STDIO = Q.store_thm("UNIQUE_STDIO",
 `!s. VALID_HEAP s ==> !fs1 fs2 H1 H2. (STDIO fs1 * H1) s /\
                                       (STDIO fs2 * H2) s ==>
-              (fs1.infds = fs2.infds /\ fs1.files = fs2.files /\
-               fs1.inode_tbl = fs2.inode_tbl)`,
+              (fs1.infds = fs2.infds /\ fs1.inode_tbl = fs2.inode_tbl /\
+               fs1.files = fs2.files)`,
   rw[STDIO_def,STD_streams_def,SEP_CLAUSES,SEP_EXISTS_THM,STAR_COMM,STAR_ASSOC,cond_STAR] >>
   fs[Once STAR_COMM] >>
   imp_res_tac UNIQUE_IOFS >>
@@ -78,7 +78,7 @@ val UNIQUE_STDIO = Q.store_thm("UNIQUE_STDIO",
 (* weak injection theorem *)
 val STDIO_HPROP_INJ = Q.store_thm("STDIO_HPROP_INJ[hprop_inj]",
 `HPROP_INJ (STDIO fs1) (STDIO fs2)
-           (fs1.infds = fs2.infds /\ fs1.files = fs2.files /\ fs1.inode_tbl = fs2.inode_tbl)`,
+           (fs1.infds = fs2.infds /\ fs1.inode_tbl = fs2.inode_tbl /\ fs1.files = fs2.files)`,
   rw[HPROP_INJ_def, GSYM STAR_ASSOC, SEP_CLAUSES, SEP_EXISTS_THM,
      HCOND_EXTRACT] >>
   EQ_TAC >> rpt DISCH_TAC
@@ -162,7 +162,7 @@ val EndOfFile_UNICITY = Q.store_thm("EndOfFile_UNICITY[xlet_auto_match]",
 val stdo_def = Define`
   stdo fd name fs out =
     (ALOOKUP fs.infds fd = SOME(UStream(strlit name),strlen out) /\
-     ALOOKUP fs.files (UStream(strlit name)) = SOME (explode out))`;
+     ALOOKUP fs.inode_tbl (UStream(strlit name)) = SOME (explode out))`;
 
 val _ = overload_on("stdout",``stdo 1 "stdout"``);
 val _ = overload_on("stderr",``stdo 2 "stderr"``);
@@ -185,12 +185,12 @@ val up_stdo_numchars = Q.store_thm("up_stdo_numchars[simp]",
   rw[up_stdo_def,fsupdate_def]
   \\ CASE_TAC \\ CASE_TAC \\ rw[]);
 
-val fsupdate_inode_tbl = Q.store_thm("fsupdate_inode_tbl",
- `(fsupdate fs fd k pos c).inode_tbl = fs.inode_tbl`,
+val fsupdate_files = Q.store_thm("fsupdate_files",
+ `(fsupdate fs fd k pos c).files = fs.files`,
  fs[fsupdate_def] >> NTAC 2 CASE_TAC >>fs[]);
 
-val up_stdo_inode_tbl = Q.store_thm("up_stdo_inode_tbl",
- `(up_stdo fd fs x).inode_tbl = fs.inode_tbl`,
+val up_stdo_files = Q.store_thm("up_stdo_files",
+ `(up_stdo fd fs x).files = fs.files`,
  fs[up_stdo_def,fsupdate_def] >> NTAC 2 CASE_TAC >>fs[]);
 
 val up_stdo_with_numchars = Q.store_thm("up_stdo_with_numchars",
@@ -253,12 +253,12 @@ val add_stdo_MAP_FST_infds = Q.store_thm("add_stdo_MAP_FST_infds[simp]",
   `MAP FST (add_stdo fd nm fs out).infds = MAP FST fs.infds`,
   rw[add_stdo_def]);
 
-val up_stdo_MAP_FST_files = Q.store_thm("up_stdo_MAP_FST_files[simp]",
-  `MAP FST (up_stdo fd fs out).files = MAP FST fs.files`,
+val up_stdo_MAP_FST_inode_tbl = Q.store_thm("up_stdo_MAP_FST_inode_tbl[simp]",
+  `MAP FST (up_stdo fd fs out).inode_tbl = MAP FST fs.inode_tbl`,
   rw[up_stdo_def]);
 
-val add_stdo_MAP_FST_files = Q.store_thm("add_stdo_MAP_FST_files[simp]",
-  `MAP FST (add_stdo fd nm fs out).files = MAP FST fs.files`,
+val add_stdo_MAP_FST_inode_tbl = Q.store_thm("add_stdo_MAP_FST_inode_tbl[simp]",
+  `MAP FST (add_stdo fd nm fs out).inode_tbl = MAP FST fs.inode_tbl`,
   rw[add_stdo_def]);
 
 val inFS_fname_add_stdo = Q.store_thm("inFS_fname_add_stdo[simp]",
@@ -365,7 +365,7 @@ val up_stdout_fastForwardFD = Q.store_thm("up_stdout_fastForwardFD",
     \\ CASE_TAC \\ fs[libTheory.the_def]
     \\ CASE_TAC \\ fs[libTheory.the_def,ALIST_FUPDKEY_ALOOKUP] )
   \\ fs[] \\ pairarg_tac \\ fs[]
-  \\ Cases_on`ALOOKUP fs.files fnm` >- (
+  \\ Cases_on`ALOOKUP fs.inode_tbl fnm` >- (
     fs[libTheory.the_def,fsupdate_def]
     \\ CASE_TAC \\ fs[libTheory.the_def]
     \\ CASE_TAC \\ fs[libTheory.the_def,ALIST_FUPDKEY_ALOOKUP]
@@ -388,7 +388,7 @@ val up_stderr_fastForwardFD = Q.store_thm("up_stderr_fastForwardFD",
     \\ CASE_TAC \\ fs[libTheory.the_def]
     \\ CASE_TAC \\ fs[libTheory.the_def,ALIST_FUPDKEY_ALOOKUP] )
   \\ fs[] \\ pairarg_tac \\ fs[]
-  \\ Cases_on`ALOOKUP fs.files fnm` >- (
+  \\ Cases_on`ALOOKUP fs.inode_tbl fnm` >- (
     fs[libTheory.the_def,fsupdate_def]
     \\ CASE_TAC \\ fs[libTheory.the_def]
     \\ CASE_TAC \\ fs[libTheory.the_def,ALIST_FUPDKEY_ALOOKUP]
@@ -412,7 +412,7 @@ val stdo_fastForwardFD = Q.store_thm("stdo_fastForwardFD",
   rw[stdo_def,fastForwardFD_def,ALIST_FUPDKEY_ALOOKUP]
   \\ Cases_on`ALOOKUP fs.infds fd` \\ fs[libTheory.the_def]
   \\ pairarg_tac \\ fs[]
-  \\ Cases_on`ALOOKUP fs.files fnm` \\ fs[libTheory.the_def]
+  \\ Cases_on`ALOOKUP fs.inode_tbl fnm` \\ fs[libTheory.the_def]
   \\ fs[ALIST_FUPDKEY_ALOOKUP] \\ rw[]
   \\ CASE_TAC);
 
@@ -446,31 +446,31 @@ val add_stderr_fastForwardFD = Q.store_thm("add_stderr_fastForwardFD",
 
 val FILTER_File_add_stdo = Q.store_thm("FILTER_File_add_stdo",
   `stdo fd nm fs init ⇒
-   FILTER (isFile o FST) (add_stdo fd nm fs out).files = FILTER (isFile o FST) fs.files`,
+   FILTER (isFile o FST) (add_stdo fd nm fs out).inode_tbl = FILTER (isFile o FST) fs.inode_tbl`,
   rw[add_stdo_def,up_stdo_def,fsupdate_def]
   \\ CASE_TAC \\ CASE_TAC \\ fs[]
   \\ match_mp_tac FILTER_EL_EQ \\ simp[]
   \\ qmatch_assum_rename_tac`_ = SOME (k,_)`
   \\ qx_gen_tac`n`
   \\ simp[GSYM AND_IMP_INTRO] \\ strip_tac
-  \\ reverse(Cases_on`FST (EL n fs.files) = k`)
+  \\ reverse(Cases_on`FST (EL n fs.inode_tbl) = k`)
   >- simp[EL_ALIST_FUPDKEY_unchanged]
   \\ simp[FST_EL_ALIST_FUPDKEY,GSYM AND_IMP_INTRO]
   \\ fs[stdo_def]);
 
 val FILTER_File_add_stdout = Q.store_thm("FILTER_File_add_stdout",
   `STD_streams fs ⇒
-   FILTER (isFile o FST) (add_stdout fs out).files = FILTER (isFile o FST) fs.files`,
+   FILTER (isFile o FST) (add_stdout fs out).inode_tbl = FILTER (isFile o FST) fs.inode_tbl`,
   metis_tac[STD_streams_stdout,FILTER_File_add_stdo]);
 
 val FILTER_File_add_stderr = Q.store_thm("FILTER_File_add_stderr",
   `STD_streams fs ⇒
-   FILTER (isFile o FST) (add_stderr fs out).files = FILTER (isFile o FST) fs.files`,
+   FILTER (isFile o FST) (add_stderr fs out).inode_tbl = FILTER (isFile o FST) fs.inode_tbl`,
   metis_tac[STD_streams_stderr,FILTER_File_add_stdo]);
 
 val stdin_def = Define
 `stdin fs inp pos = (ALOOKUP fs.infds 0 = SOME(UStream(strlit"stdin"),pos) /\
-                     ALOOKUP fs.files (UStream(strlit"stdin"))= SOME inp)`
+                     ALOOKUP fs.inode_tbl (UStream(strlit"stdin"))= SOME inp)`
 
 val up_stdin_def = Define
 `up_stdin inp pos fs = fsupdate fs 0 0 pos inp`
@@ -1879,7 +1879,7 @@ val inputLinesFrom_spec = Q.store_thm("inputLinesFrom_spec",
   \\ qmatch_assum_abbrev_tac`validFD fd fso`
   \\ `∃c. get_file_content fso fd = SOME (c,0)`
   by (
-    fs[get_file_content_def,validFD_def,Abbr`fso`,openFileFS_files]
+    fs[get_file_content_def,validFD_def,Abbr`fso`,openFileFS_inode_tbl]
     \\ imp_res_tac inFS_fname_ALOOKUP_EXISTS \\ fs[] \\ rw[])
   \\ xlet_auto >- xsimpl
   \\ qmatch_goalsub_abbrev_tac`STDIO fsob`
@@ -1896,14 +1896,14 @@ val inputLinesFrom_spec = Q.store_thm("inputLinesFrom_spec",
   \\ fs[all_lines_def,lines_of_def]
   \\ fs[get_file_content_def]
   \\ pairarg_tac \\ fs[]
-  \\ fs[Abbr`fso`,openFileFS_files]
+  \\ fs[Abbr`fso`,openFileFS_inode_tbl]
   \\ rveq \\ fs[]
   \\ qmatch_goalsub_abbrev_tac`STDIO fs'`
   \\ `fs' = fs` suffices_by ( rw[] \\ xsimpl)
   \\ unabbrev_all_tac
   \\ simp[fastForwardFD_def,A_DELKEY_ALIST_FUPDKEY,o_DEF,
-          libTheory.the_def, openFileFS_numchars,openFileFS_inode_tbl,
-          IO_fs_component_equality,openFileFS_files]);
+          libTheory.the_def, openFileFS_numchars,openFileFS_files,
+          IO_fs_component_equality,openFileFS_inode_tbl]);
 
 val inputLinesFrom_def = Define `
   inputLinesFrom f =
