tutorial/wordcountProgScript.sml
@@ -31,7 +31,7 @@ val wordcount_spec = Q.store_thm("wordcount_spec",
   `hasFreeFD fs ∧
    cl = [pname; fname] ∧
    ALOOKUP fs.file_inode fname = SOME ino ∧
-   ALOOKUP fs.files (File ino) = SOME contents
+   ALOOKUP fs.inode_tbl (File ino) = SOME contents
    ⇒
    app (p:'ffi ffi_proj) ^(fetch_v "wordcount" (get_ml_prog_state()))
      [uv] (STDIO fs * COMMANDLINE cl)
